exercises/pure.v
@@ -16,29 +16,15 @@ Local Notation "Q ⊢ P" := (Q ⊢@{iPropI Σ} P).
 (** * Pure Propositions *)
 
 (**
-  The implementation of Iris in Coq has a unique class of propositions
-  called `pure'. This class arises from the fact that Coq propositions
-  can be embedded into the logic of Iris. Any Coq proposition [φ : Prop]
-  can be turned into an Iris proposition through the pure embedding
-  [⌜φ⌝ : iProp Σ]. This allows us to piggyback on much of the
-  functionality and theory developed for the logic of Coq. The
-  proposition [⌜φ⌝] is thus an Iris proposition, and we can use it as we
-  would any other Iris proposition.
+  Any Rocq proposition [φ : Prop] can be turned into an Iris proposition through
+  the pure embedding [⌜φ⌝ : iProp Σ] (type \lc and \rc). We call these
+  "pure assertions".
 *)
 
-Lemma asm_pure (φ : Prop) : ⌜φ⌝ ⊢ ⌜φ⌝.
-Proof.
-  iIntros "H".
-  iApply "H".
-Qed.
-
 (**
-  A pure proposition is then any Iris proposition [P] for which there
-  exists a Coq proposition [φ], such that [P ⊣⊢ ⌜φ⌝].
-
   Pure propositions can be introduced using [iPureIntro]. This exits the
   Iris Proof Mode, throwing away the spatial context and turns the
-  proposition into a Coq proposition.
+  proposition into a Rocq proposition.
 *)
 Lemma eq_5_5 : ⊢ ⌜5 = 5⌝.
 Proof.
@@ -48,7 +34,7 @@ Qed.
 
 (**
   To eliminate a pure proposition, we can use the specialization pattern
-  ["%_"]. This adds the proposition to the non-spatial context as a Coq
+  ["%_"]. This adds the proposition to the non-spatial context as a Rocq
   proposition.
 *)
 Lemma eq_elm {A} (P : A → iProp Σ) (x y : A) : ⌜x = y⌝ -∗ P x -∗ P y.
@@ -57,15 +43,6 @@ Proof.
   rewrite -Heq.
   iApply "HP".
 Qed.
-
-(**
-  It is quite easy to show that the propositions [⌜5 = 5⌝] and [⌜x = y⌝]
-  from above are pure. However, it can become quite burdensome for more
-  complicated Iris propositions. Fortunately, Iris has two typeclasses
-  [IntoPure] and [FromPure] that can identify pure propositions for us.
-  These are used by the [iPureIntro] tactic to identify pure
-  propositions automatically.
-*)
 
 (** [True] is pure. *)
 Lemma true_intro : ⊢ True.
@@ -110,12 +87,12 @@ Qed.
   The pure embedding allows us to state an important property, namely
   soundness. Soundness is proved in the [uPred_primitive.pure_soundness]
   lemma stating: [∀ φ, (True ⊢ ⌜φ⌝) → φ]. This means that anything
-  proved inside the Iris logic is as true as anything proved in Coq.
+  proved inside the Iris logic is as true as anything proved in Rocq.
 *)
 
 (**
-  [⌜_⌝] turns Coq propositions into Iris propositions, while [⊢ _] turns
-  Iris propositions into Coq propositions. These operations are not
+  [⌜_⌝] turns Rocq propositions into Iris propositions, while [⊢ _] turns
+  Iris propositions into Rocq propositions. These operations are not
   inverses, but they are related.
 *)
 Lemma pure_adj1 (φ : Prop) : φ → ⊢ ⌜φ⌝.
